---
layout: page
title: 2019 A1
description: A problem about determining possible values from a given expression.
img: assets/img/2019_A1.png
importance: 2
category: Number Theory
related_publications: false
permalink: /Putnam_Problems/2019_A1/
---

<!-- Inline styling for larger text in Google Sites -->
<div style="font-size: 20px; line-height: 1.5;">

<!-- Begin solution -->
<p>Last updated 9/21/25</p>
<h2 id="problem-setup">Problem Setup</h2>
<p>Determine all possible values of the expression <span
class="math display">\[\begin{equation*}
    A^3 + B^3 +C^3 -3ABC
\end{equation*}\]</span> where <span class="math inline">\(A,
B,\)</span> and <span class="math inline">\(C\)</span> are nonnegative
integers.</p>
<h2 id="solution">Solution</h2>
<p>Without loss of generality, we can assert that <span
class="math display">\[\begin{equation*}
    A \ge B \ge C
\end{equation*}\]</span> since <span class="math inline">\(A,B\)</span>
and <span class="math inline">\(C\)</span> are exchangeable in the given
expression. For example, if we have <span
class="math inline">\(A=1\)</span>, <span
class="math inline">\(B=1\)</span>, and <span
class="math inline">\(C=3\)</span>, we can just switch the labels of
<span class="math inline">\(A\)</span> and <span
class="math inline">\(C\)</span> without changing the value of the
expression. This is true for all <span class="math inline">\(A,\)</span>
<span class="math inline">\(B,\)</span> and <span
class="math inline">\(C\)</span>.</p>
<p>Let <span class="math inline">\(B=A-b\)</span> and <span
class="math inline">\(C = A-c\)</span>, with <span
class="math inline">\(b,c \in \mathbb{N}\)</span> and <span
class="math inline">\(b \ge c \ge 0\)</span> and <span
class="math inline">\(A \ge b\)</span> (otherwise our asserted ordering
fails). Then, the original expression becomes <span
class="math display">\[\begin{align*}
    A^3 + (A-b)^3 + (A-c)^3 -3A(A-b)(A-c) &amp;=
3Ab^2-3Abc+3Ac^2-b^3-c^3 \\
    &amp;= 3A(b^2-bc+c^2) - (b^3-c^3)
\end{align*}\]</span> Weâ€™ll denote this expression <span
class="math inline">\(E\)</span>. For <span
class="math inline">\(b=1\)</span> and <span
class="math inline">\(c=0\)</span> (assuming <span
class="math inline">\(A\ge1\)</span>): <span
class="math display">\[\begin{equation}
    E=3A(1)-(1) = 3A-1
\end{equation}\]</span> For <span class="math inline">\(b=c=1\)</span>
(still with <span class="math inline">\(A\ge1)\)</span>: <span
class="math display">\[\begin{equation}
    E=3A(1-1+1)-(1+1) = 3A-2
\end{equation}\]</span> For <span class="math inline">\(b=2\)</span> and
<span class="math inline">\(c=1\)</span>, assuming <span
class="math inline">\(A\ge2\)</span>: <span
class="math display">\[\begin{equation}
    E=3A(4-2+1)-(8+1) = 9(A-1)
\end{equation}\]</span> Considering expressions 1, 2, and 3, we can
realize a few groups of possible values. Expressions 1 and 2 guarantee
all integers that are not a multiple of 3, and expression 3 guarantees
all integers that are a multiple of 9. In the next section, we will show
that these are the only possible integers for the given expression.</p>
<p>To determine what multiples of 3, if any, are possible, we need to
find the <span class="math inline">\(b\)</span> and <span
class="math inline">\(c\)</span> that causes <span
class="math inline">\(E=3A(b^2-bc+c^2)-(b^3 + c^3)\)</span> to be a
multiple of 3. Since the first term is already a multiple of 3, we only
really need to determine when <span class="math inline">\(b^3 +c^3
\equiv0\)</span> (mod 3) is true. If <span class="math inline">\(b\equiv
c \equiv0\)</span> (mod 3), then <span
class="math display">\[\begin{align*}
    E = 3A\Bigg( 3^2\Big(\frac{b}{3} \Big)^2 - 3^2 \Big( \frac{bc}{3^2}
\Big) +3^2 \Big( \frac{c}{3} \Big)^2 \Bigg) -3^3\Bigg( \Big( \frac{b}{3}
\Big)^3 + \Big( \frac{c}{3} \Big)^3 \Bigg)
\end{align*}\]</span> and so <span class="math inline">\(E\)</span> is a
multiple of 9. The only other choice of <span
class="math inline">\(b\)</span> and <span
class="math inline">\(c\)</span> is <span
class="math inline">\(b\equiv1\)</span> (mod 3) and <span
class="math inline">\(c\equiv2\)</span> (mod 3), or vice versa, since it
is the only remaining combination that still gives <span
class="math inline">\(b^3+c^3 \equiv0\)</span> (mod 3). We then have
<span class="math display">\[\begin{align*}
    E &amp;= 3A\Big( (3x+1)^2 -(3x+1)(3y+2) +(3y+2)^2 \Big) - \Big(
(3x+1)^3 + (3y+2)^3 \Big) \\
    &amp;= 3A\Big( (3x+1)^2 -(3x+1)(3y+2) +(3y+2)^2 \Big) - \Big( 9r+9
\Big)
\end{align*}\]</span> In the first term, we can note that <span
class="math inline">\((3x+1)^2 \equiv (3y+2)^2 \equiv 1\)</span> (mod 3)
and <span class="math inline">\((3x+1)(3y+2) \equiv 2\)</span> (mod 3),
so the sum <span class="math inline">\((3x+1)^2 -(3x+1)(3y+2) + (3y+2)^2
\equiv 0\)</span> (mod 3), making the first term also a multiple of 9.
Therefore, the only choices of <span class="math inline">\(b\)</span>
and <span class="math inline">\(c\)</span> that make the expression
<span class="math inline">\(E\)</span> a multiple of 3 also force it to
be a multiple of 9.</p>
<p>Finally, we can say that the only possible values of <span
class="math inline">\(A^3+B^3+C^3 -3ABC\)</span> are <strong>all
nonnegative integers except those that are 3 or 6 (mod 9)</strong>.</p>

 
</div>

<!-- MathJax Configuration to Scale Font Size for Math -->
<script type="text/javascript">
  window.MathJax = {
    tex: {
      inlineMath: [['$', '$'], ['\\(', '\\)']]
    },
    chtml: {
      scale: 0.5  // Scale up the math font size
    }
  };
</script>

<!-- MathJax Script -->
<script type="text/javascript" async
  src="https://cdnjs.cloudflare.com/ajax/libs/mathjax/3.2.0/es5/tex-mml-chtml.js">
</script>

